WIP
WIP

WIP

WIP

WIP

WIP

WIP

WIP

WIP

WIP

WIP

WIP

WIP

Broken WIP

Revert "Broken WIP"

This reverts commit f0bbba2ff60cda497234b73ea51a7651eae9a23a.

WIP

WIP

WIP

WIP

WIP

WIP

WIP

WIP

WIP

WIP

WIP

WIP

WIP

WIP

Use Z.mul_split_cps, not Z.mul_split_cps'

WIP

Use Z.mul_split_cps, not Z.mul_split_cps'

WIP

WIP

WIP

Revert "WIP"

This reverts commit 195bc2218329b455086e02c61c4a4ed368199659.

Revert "Revert "WIP""

This reverts commit d2f3fd501b0303261fc734ead378ccbe59cdaf1e.

WIP

WIP

WIP

WIP

WIP

WIP

WIP

WIP

WIP

WIP

WIP

WIP

WIP

WIP

WIP

WIP

WIP

WIP

WIP

WIP

WIP

WIP

WIP

WIP

WIP

WIP

WIP

WIP

WIP

WIP

WIP

WIP

WIP

WIP

WIP

WIP

WIP

WIP

WIP

WIP

WIP

WIP

WIP

WIP

WIP

WIP

WIP

WIP

WIP

WIP

WIP

WIP

WIP correct encode decode for mont

WIP

WIP

WIP

WIP

WIP

WIP

WIP

WIP

WIP

WIP

WIP

WIP

WIP

src/Arithmetic/CoreUnfolder_bak.v
@@ -3,24 +3,23 @@ Require Import Crypto.Util.LetIn.
 Require Import Crypto.Util.ZUtil.Definitions.
 Require Import Crypto.Util.ZUtil.CPS.
 Require Import Crypto.Util.IdfunWithAlt.
-Require Import Crypto.Util.CPSUtil.
 Require Import Crypto.Arithmetic.Core.
 Require Import Crypto.Util.Tactics.VM.
 
 Create HintDb arithmetic_cps_unfolder.
-Create HintDb parameterized_sig_unfolder discriminated.
 
 Hint Unfold Core.div Core.modulo : arithmetic_cps_unfolder.
 
 Ltac make_parameterized_sig t :=
   refine (_ : { v : _ | v = t });
-  eexists; repeat autounfold with parameterized_sig_unfolder;
+  eexists;
+  cbv delta [t];
+  repeat autounfold with basesystem_partial_evaluation_unfolder arithmetic_cps_unfolder;
   cbv delta [t
-               Core.B.Positional.chained_carries_reduce_cps_step
                B.limb ListUtil.sum ListUtil.sum_firstn
                CPSUtil.Tuple.mapi_with_cps CPSUtil.Tuple.mapi_with'_cps CPSUtil.flat_map_cps CPSUtil.on_tuple_cps CPSUtil.fold_right_cps2
                Decidable.dec Decidable.dec_eq_Z
-               id_tuple_with_alt id_tuple'_with_alt id_tuple_with_alt_cps'
+               id_tuple_with_alt id_tuple'_with_alt
                Z.add_get_carry_full Z.mul_split
                Z.add_get_carry_full_cps Z.mul_split_cps Z.mul_split_cps'
                Z.add_get_carry_cps];
@@ -29,15 +28,75 @@ Ltac make_parameterized_sig t :=
 
 Notation parameterize_sig t := ltac:(let v := t in make_parameterized_sig v) (only parsing).
 
+Ltac refresh x :=
+  let maybe_x := fresh x in
+  let maybe_x := fresh x in
+  let maybe_x := fresh x in
+  let not_x := fresh x in
+  not_x.
+Ltac pattern_let_in_tuple_under_binders t Z let_inZ let_inZZ :=
+  match t with
+  | (fun x : nat => _)
+    => let x' := refresh x in
+       let ret
+           := constr:(
+                fun x' : nat
+                => ltac:(
+                     let v := (eval cbv beta in (t x')) in
+                     lazymatch v with
+                     | context[Tuple.tuple _ x']
+                       => let v := (eval pattern (@Let_In Z (fun _ => Tuple.tuple Z x')),
+                                    (@Let_In (Z * Z)%type (fun _ => Tuple.tuple Z x'))
+                                     in v) in
+                          let v := match v with ?v _ _ => v end in
+                          let v := (eval cbv beta in (v (let_inZ x') (let_inZZ x'))) in
+                          exact v
+                     end)) in
+       ret
+  | (fun x : ?X => _)
+    => let x' := refresh x in
+       let ret
+           := constr:(
+                fun x' : X
+                => ltac:(
+                     let v := (eval cbv beta in (t x')) in
+                     let v := pattern_let_in_tuple_under_binders v Z let_inZ let_inZZ in
+                     exact v)) in
+       ret
+  end.
+
+Ltac pattern_strip_full_extra t :=
+  let t := (eval cbv beta in (t Z (@LetIn.Let_In))) in
+  let t := constr:(fun (let_inZ : forall n, Z -> (Z -> Tuple.tuple Z n) -> Tuple.tuple Z n)
+                       (let_inZZ : forall n, Z * Z -> (Z * Z -> Tuple.tuple Z n) -> Tuple.tuple Z n)
+                   => ltac:(let liZ := constr:(let_inZ) in
+                            let liZZ := constr:(let_inZZ) in
+                            let v := match t with
+                                     | _ => pattern_let_in_tuple_under_binders t Z liZ liZZ
+                                     | _ => t
+                                     end in
+                            exact v)) in
+  let t := (eval pattern Z, (@Let_In) in t) in
+  let t := match t with ?t _ _ => t end in
+  t.
+Ltac apply_patterned_full_extra t :=
+  eval cbv beta in
+    (fun Z Let_In
+     => t Z Let_In
+          (fun n : nat => @Let_In Z (fun _ => Tuple.tuple Z n))
+          (fun n : nat => @Let_In (Z * Z)%type (fun _ => Tuple.tuple Z n))).
+
 Ltac make_parameterized_from_sig t_sig :=
   let t := (eval cbv [proj1_sig t_sig] in (proj1_sig t_sig)) in
-  let t := pattern_strip t in
+  let t := pattern_strip_full t in
+  let t := pattern_strip_full_extra t in
   exact t.
 
 Notation parameterize_from_sig t := ltac:(let v := t in make_parameterized_from_sig v) (only parsing).
 
 Ltac make_parameterized_eq t t_sig :=
-  let t := apply_patterned t in
+  let t := apply_patterned_full_extra t in
+  let t := apply_patterned_full t in
   exact (proj2_sig t_sig : t = _).
 
 Notation parameterize_eq t t_sig := ltac:(let v := t in let v_sig := t_sig in make_parameterized_eq v v_sig) (only parsing).
@@ -66,7 +125,7 @@ for i in eval multerm mul_cps mul split_cps split reduce_cps reduce negate_snd_c
 done
 echo "  End Associational."
 echo "  Module Positional."
-for i in to_associational_cps to_associational eval zeros add_to_nth_cps add_to_nth place_cps place from_associational_cps from_associational carry_cps carry chained_carries_cps chained_carries encode add_cps mul_cps reduce_cps carry_reduce_cps  chained_carries_reduce_cps_step chained_carries_reduce_cps chained_carries_reduce negate_snd_cps split_cps scmul_cps unbalanced_sub_cps sub_cps sub opp_cps Fencode Fdecode eval_from select_cps select; do
+for i in to_associational_cps to_associational eval zeros add_to_nth_cps add_to_nth place_cps place from_associational_cps from_associational carry_cps carry chained_carries_cps chained_carries encode add_cps mul_cps reduce_cps carry_reduce_cps negate_snd_cps split_cps scmul_cps unbalanced_sub_cps sub_cps sub opp_cps Fencode Fdecode eval_from select_cps select; do
   echo "    Definition ${i}_sig := parameterize_sig (@Core.B.Positional.${i}).";
   echo "    Definition ${i} := parameterize_from_sig ${i}_sig.";
   echo "    Definition ${i}_eq := parameterize_eq ${i} ${i}_sig.";
@@ -283,24 +342,6 @@ done
     Definition carry_reduce_cps_eq := parameterize_eq carry_reduce_cps carry_reduce_cps_sig.
     Hint Unfold carry_reduce_cps : basesystem_partial_evaluation_unfolder.
     Hint Rewrite <- carry_reduce_cps_eq : pattern_runtime.
-
-    Definition chained_carries_reduce_cps_step_sig := parameterize_sig (@Core.B.Positional.chained_carries_reduce_cps_step).
-    Definition chained_carries_reduce_cps_step := parameterize_from_sig chained_carries_reduce_cps_step_sig.
-    Definition chained_carries_reduce_cps_step_eq := parameterize_eq chained_carries_reduce_cps_step chained_carries_reduce_cps_step_sig.
-    Hint Unfold chained_carries_reduce_cps_step : basesystem_partial_evaluation_unfolder.
-    Hint Rewrite <- chained_carries_reduce_cps_step_eq : pattern_runtime.
-
-    Definition chained_carries_reduce_cps_sig := parameterize_sig (@Core.B.Positional.chained_carries_reduce_cps).
-    Definition chained_carries_reduce_cps := parameterize_from_sig chained_carries_reduce_cps_sig.
-    Definition chained_carries_reduce_cps_eq := parameterize_eq chained_carries_reduce_cps chained_carries_reduce_cps_sig.
-    Hint Unfold chained_carries_reduce_cps : basesystem_partial_evaluation_unfolder.
-    Hint Rewrite <- chained_carries_reduce_cps_eq : pattern_runtime.
-
-    Definition chained_carries_reduce_sig := parameterize_sig (@Core.B.Positional.chained_carries_reduce).
-    Definition chained_carries_reduce := parameterize_from_sig chained_carries_reduce_sig.
-    Definition chained_carries_reduce_eq := parameterize_eq chained_carries_reduce chained_carries_reduce_sig.
-    Hint Unfold chained_carries_reduce : basesystem_partial_evaluation_unfolder.
-    Hint Rewrite <- chained_carries_reduce_eq : pattern_runtime.
 
     Definition negate_snd_cps_sig := parameterize_sig (@Core.B.Positional.negate_snd_cps).
     Definition negate_snd_cps := parameterize_from_sig negate_snd_cps_sig.
