src/Specific/Framework/ArithmeticSynthesis/Ladderstep.v
@@ -1,4 +1,5 @@
 Require Import Coq.ZArith.BinIntDef.
+Require Import Coq.Classes.Morphisms.
 Require Import Crypto.Arithmetic.Core. Import B.
 Require Import Crypto.Arithmetic.PrimeFieldTheorems.
 Require Import Crypto.Curves.Montgomery.XZ.
@@ -8,7 +9,9 @@ Require Import Crypto.Util.LetIn.
 Require Import Crypto.Util.Notations.
 Require Import Crypto.Util.Tactics.PoseTermWithName.
 Require Import Crypto.Util.Tactics.CacheTerm.
+Require Import Crypto.Util.Tactics.DestructHead.
 Require Import Crypto.Util.Option.
+Require Import Crypto.Util.Notations.
 
 Local Notation tuple := Tuple.tuple.
 Local Open Scope list_scope.
@@ -19,39 +22,121 @@ Local Infix "^" := tuple : type_scope.
 Definition FMxzladderstep {m} := @M.donnaladderstep (F m) F.add F.sub F.mul.
 
 Section with_notations.
-  Context sz (add sub mul : tuple Z sz -> tuple Z sz -> tuple Z sz)
-          (square carry : tuple Z sz -> tuple Z sz).
+  Context (T_tight T_loose : Type).
+  Local Notation retT := (tuple (tuple T_tight 2) 2).
+  Context (relax : T_tight -> T_loose)
+          (let_inT : T_tight -> (T_tight -> retT) -> retT)
+          (let_inL : T_loose -> (T_loose -> retT) -> retT)
+          (add sub : T_tight -> T_tight -> T_loose)
+          (carry_mul : T_loose -> T_loose -> T_tight)
+          (carry_square : T_loose -> T_tight).
   Local Infix "+" := add.
-  Local Notation "a * b" := (carry (mul a b)).
-  Local Notation "x ^ 2" := (carry (square x)).
+  Local Notation "a * b" := (carry_mul a b).
+  Local Notation "x ^ 2" := (carry_square x).
   Local Infix "-" := sub.
+  Local Notation "'dlet' x .. y := v 'in' f" := (let_inT v (fun x => .. (fun y => f) .. )).
+  Local Notation "'llet' x := v 'in' f" := (let_inL v (fun x => f)).
+  Local Coercion relax : T_tight >-> T_loose.
   Definition Mxzladderstep a24 x1 Q Q'
     := match Q, Q' with
        | (x, z), (x', z') =>
          dlet origx := x in
-         dlet x := x + z in
-         dlet z := origx - z in
+         llet x := x + z in
+         llet z := origx - z in
          dlet origx' := x' in
-         dlet x' := x' + z' in
-         dlet z' := origx' - z' in
+         llet x' := x' + z' in
+         llet z' := origx' - z' in
          dlet xx' := x' * z in
          dlet zz' := x * z' in
          dlet origx' := xx' in
-         dlet xx' := xx' + zz' in
-         dlet zz' := origx' - zz' in
+         llet xx' := xx' + zz' in
+         llet zz' := origx' - zz' in
          dlet x3 := xx'^2 in
          dlet zzz' := zz'^2 in
          dlet z3 := zzz' * x1 in
          dlet xx := x^2 in
          dlet zz := z^2 in
          dlet x2 := xx * zz in
-         dlet zz := xx - zz in
+         llet zz := xx - zz in
          dlet zzz := zz * a24 in
-         dlet zzz := zzz + xx in
+         llet zzz := zzz + xx in
          dlet z2 := zz * zzz in
          ((x2, z2), (x3, z3))%core
        end.
+
+
+  Lemma Mxzladderstep_Proper1
+        (P_tight : T_tight -> Prop)
+        (P_loose : T_loose -> Prop)
+        (P_ret : tuple (tuple T_tight 2) 2 -> Prop
+         := fun x => (P_tight (fst (fst x)) /\ P_tight (snd (fst x)))
+                     /\ (P_tight (fst (snd x)) /\ P_tight (snd (snd x))))
+        (P_relax : forall x, P_tight x -> P_loose (relax x))
+        (P_let_inT : forall x (_ : P_tight x) f (_ : forall x, P_tight x -> P_ret (f x)), P_ret (let_inT x f))
+        (P_let_inL : forall x (_ : P_loose x) f (_ : forall x, P_loose x -> P_ret (f x)), P_ret (let_inL x f))
+        (P_add : forall x (_ : P_tight x) y (_ : P_tight y), P_loose (add x y))
+        (P_sub : forall x (_ : P_tight x) y (_ : P_tight y), P_loose (sub x y))
+        (P_carry_mul : forall x (_ : P_loose x) y (_ : P_loose y), P_tight (carry_mul x y))
+        (P_carry_square : forall x (_ : P_loose x), P_tight (carry_square x))
+        a24 x1 Q Q'
+        (P_a24 : P_loose a24)
+        (P_x1 : P_loose x1)
+        (P_Q : P_tight (fst Q) /\ P_tight (snd Q))
+        (P_Q' : P_tight (fst Q') /\ P_tight (snd Q'))
+    : P_ret (Mxzladderstep a24 x1 Q Q').
+  Proof.
+    destruct Q, Q', P_Q, P_Q'; cbv [Mxzladderstep]; cbn [fst snd] in *.
+    repeat match goal with
+           | [ H : _ |- _ ] => apply H; repeat intro; try assumption
+           | _ => progress repeat apply conj; try assumption
+           end.
+  Qed.
 End with_notations.
+
+Section hetero.
+  Local Notation "f ==> g"
+    := (respectful_hetero _ _ (fun _ => _) (fun _ => _) f%signature (fun _ _ => g%signature)) : signature_scope.
+  Local Notation "R ^ n" := (Tuple.fieldwise (n:=n%nat) R%signature) : signature_scope.
+  Local Notation "R ^ 2" := (Tuple.fieldwise (n:=2) R%signature) : signature_scope.
+
+  Lemma Mxzladderstep_Proper_hetero
+        {T1_tight T1_loose T2_tight T2_loose}
+        (R_tight : T1_tight -> T2_tight -> Prop)
+        (R_loose : T1_loose -> T2_loose -> Prop)
+    : (((R_tight ==> R_loose)
+          ==> (R_tight ==> (R_tight ==> (R_tight^2)^2) ==> (R_tight^2)^2)
+          ==> (R_loose ==> (R_loose ==> (R_tight^2)^2) ==> (R_tight^2)^2)
+          ==> (R_tight ==> R_tight ==> R_loose)
+          ==> (R_tight ==> R_tight ==> R_loose)
+          ==> (R_loose ==> R_loose ==> R_tight)
+          ==> (R_loose ==> R_tight)
+          ==> R_loose
+          ==> R_loose
+          ==> (R_tight^2)
+          ==> (R_tight^2)
+          ==> (R_tight^2)^2)%signature)
+        (@Mxzladderstep T1_tight T1_loose)
+        (@Mxzladderstep T2_tight T2_loose).
+  Proof.
+    cbv [tuple tuple']; repeat intro; destruct_head'_prod;
+      destruct_head_hnf' and;
+      cbn [fst snd] in *; cbv [fieldwise'] in *.
+    cbv [Mxzladderstep].
+    repeat match goal with
+           | _ => progress repeat intro
+           | [ H : _ |- _ ] => apply H; try assumption
+           | _ => progress repeat apply conj; cbn [fst snd]; try assumption
+           end.
+  Qed.
+End hetero.
+
+Definition FMxzladderstep_Mxzladderstep {m}
+  : @FMxzladderstep m
+    = @Mxzladderstep (F m) (F m) id (@Let_In _ _) (@Let_In _ _) F.add F.sub F.mul (fun x => F.mul x x)
+  := eq_refl.
+
+
+(*
 
 Ltac pose_a24' a24 a24' :=
   let a24 := (eval vm_compute in (invert_Some a24)) in
@@ -85,3 +170,4 @@ Ltac pose_Mxzladderstep_sig sz wt m add_sig sub_sig mul_sig square_sig carry_sig
                  end;
           reflexivity)
            Mxzladderstep_sig.
+*)
