src/Specific/Framework/ArithmeticSynthesis/Montgomery.v
@@ -2,8 +2,18 @@ Require Import Coq.micromega.Lia.
 Require Import Crypto.Arithmetic.MontgomeryReduction.WordByWord.Definition.
 Require Import Crypto.Arithmetic.MontgomeryReduction.WordByWord.Proofs.
 Require Import Crypto.Arithmetic.Core. Import B.
+Require Import Crypto.Arithmetic.ModularArithmeticTheorems.
 Require Crypto.Arithmetic.Saturated.MontgomeryAPI.
 Require Import Crypto.Arithmetic.Saturated.UniformWeight.
+Require Crypto.Specific.Framework.CurveParameters.
+Require Import Crypto.Specific.Framework.ArithmeticSynthesis.Base.
+Require Import Crypto.Compilers.Syntax.
+Require Import Crypto.Compilers.Z.Syntax.
+Require Import Crypto.Compilers.Z.Reify.
+Require Import Crypto.Compilers.ExprInversion.
+Require Import Crypto.Compilers.Tuple.
+Require Import Crypto.Arithmetic.Compiled.Core.
+Require Import Crypto.Arithmetic.Compiled.Saturated.Montgomery.
 Require Import Crypto.Util.Sigma.Lift.
 Require Import Coq.ZArith.BinInt.
 Require Import Coq.PArith.BinPos.
@@ -12,13 +22,22 @@ Require Import Crypto.Util.ZUtil.ModInv.
 Require Import Crypto.Util.ZUtil.Tactics.PullPush.Modulo.
 Require Import Crypto.Util.Tactics.DestructHead.
 Require Import Crypto.Util.Tactics.BreakMatch.
+Require Import Crypto.Util.Option.
+Require Import Crypto.Util.ZUtil.Tactics.LtbToLt.
 Require Import Crypto.Util.Decidable.
 Require Import Crypto.Arithmetic.Saturated.UniformWeightInstances.
 Require Import Crypto.Specific.Framework.ArithmeticSynthesis.HelperTactics.
+Require Import Crypto.Util.SideConditions.CorePackages.
+Require Import Crypto.Util.SideConditions.ModInvPackage.
+Require Import Crypto.Util.SideConditions.AdmitPackage.
+Require Import Crypto.Util.SideConditions.ReductionPackages.
 Require Import Crypto.Util.Tactics.CacheTerm.
-
 Local Open Scope Z_scope.
 Local Infix "^" := Tuple.tuple : type_scope.
+
+Local Set Implicit Arguments.
+
+Local Existing Instance Tuple.dec_eq'.
 
 Local Definition sig_by_eq {A P} (x : { a : A | P a }) (a : A) (H : a = proj1_sig x)
   : { a : A | P a }.
@@ -83,6 +102,34 @@ Section with_args.
   Definition montgomery_to_F_gen (v : Z) : F m
     := (F.of_Z m v * F.of_Z m (r'^Z.of_nat sz)%Z)%F.
 
+  Definition montgomery_of_F_gen (v : F m) : Z
+    := F.to_Z (v * F.of_Z m (r^Z.of_nat sz))%F.
+
+  Lemma montgomery_to_F_of_F_gen v
+    : montgomery_to_F_gen (montgomery_of_F_gen v) = v.
+  Proof.
+    cbv [montgomery_to_F_gen montgomery_of_F_gen].
+    rewrite F.of_Z_to_Z, <- (F.of_Z_to_Z v), F.eq_to_Z_iff.
+    autorewrite with pull_FofZ.
+    rewrite <- Z.mul_assoc, !F.to_Z_of_Z, (Z.mul_comm (Z.pos r ^ _)), <- Z.pow_mul_l.
+    push_Zmod.
+    rewrite Z.pow_mul_l, m_enc_correct_montgomery, r'_pow_correct, <- m_enc_correct_montgomery, Z.mul_1_r.
+    pull_Zmod.
+    reflexivity.
+  Qed.
+
+  Lemma montgomery_of_F_gen_bounded (v : F m)
+    : 0 <= montgomery_of_F_gen v < Z.pos r ^ Z.of_nat sz.
+  Proof.
+    cbv [montgomery_of_F_gen].
+    rewrite <- F.mod_to_Z.
+    split; [ | etransitivity ];
+      [ apply Z.mod_pos_bound; lia.. | ].
+    rewrite m_enc_correct_montgomery.
+    apply MontgomeryAPI.eval_small; [ lia | ].
+    apply m_enc_small.
+  Qed.
+
   Local Definition mul_ext_gen
     : { f:Z^sz -> Z^sz -> Z^sz
       | let eval := MontgomeryAPI.eval (Z.pos r) in
@@ -92,17 +139,20 @@ Section with_args.
             = (montgomery_to_F_gen (eval A) * montgomery_to_F_gen (eval B))%F)
         /\ (forall (A : Z^sz) (_ : small (Z.pos r) A)
                    (B : Z^sz) (_ : small (Z.pos r) B),
-               (eval B < eval m_enc -> 0 <= eval (f A B) < eval m_enc)%Z) }.
+               (eval B < eval m_enc -> 0 <= eval (f A B) < eval m_enc)%Z)
+        /\ (forall (A : Z^sz) (_ : small (Z.pos r) A)
+                   (B : Z^sz) (_ : small (Z.pos r) B),
+               small (Z.pos r) (f A B)) }.
   Proof.
     exists (proj1_sig mul'_gen).
     abstract (
-        split; intros A Asm B Bsm;
+        cbv zeta; intros; repeat apply conj; intros A Asm B Bsm;
         pose proof (proj2_sig mul'_gen A B Asm Bsm) as H;
         cbv zeta in *;
         try solve [ destruct_head'_and; assumption ];
         rewrite ModularArithmeticTheorems.F.eq_of_Z_iff in H;
         unfold montgomery_to_F_gen;
-        destruct H as [H1 [H2 H3]];
+        destruct H as [H1 [H2 H3]]; trivial;
         rewrite H3;
         rewrite <- !ModularArithmeticTheorems.F.of_Z_mul;
         f_equal; nia
@@ -122,15 +172,21 @@ Section with_args.
                     (B : Z^sz) (_ : small (Z.pos r) B),
                 (eval A < eval m_enc
                  -> eval B < eval m_enc
-                 -> 0 <= eval (f A B) < eval m_enc)))%Z }.
+                 -> 0 <= eval (f A B) < eval m_enc))
+         /\ (forall (A : Z^sz) (_ : small (Z.pos r) A)
+                    (B : Z^sz) (_ : small (Z.pos r) B),
+                (eval A < eval m_enc
+                 -> eval B < eval m_enc
+                 -> small (Z.pos r) (f A B))))%Z }.
   Proof.
     exists (fun A B => add (r:=r)(R_numlimbs:=sz) m_enc A B).
     abstract (
-        split; intros;
+        cbv zeta; repeat apply conj; intros;
         unfold montgomery_to_F_gen; rewrite <- ?ModularArithmeticTheorems.F.of_Z_mul, <- ?ModularArithmeticTheorems.F.of_Z_add;
         rewrite <- ?Z.mul_add_distr_r;
         [ rewrite <- ModularArithmeticTheorems.F.eq_of_Z_iff, m_enc_correct_montgomery; push_Zmod; rewrite eval_add_mod_N; pull_Zmod
-        | apply add_bound ];
+        | apply add_bound
+        | apply small_add ];
         t_fin
       ).
   Defined.
@@ -148,15 +204,21 @@ Section with_args.
                     (B : Z^sz) (_ : small (Z.pos r) B),
                 (eval A < eval m_enc
                  -> eval B < eval m_enc
-                 -> 0 <= eval (f A B) < eval m_enc)))%Z }.
+                 -> 0 <= eval (f A B) < eval m_enc))
+         /\ (forall (A : Z^sz) (_ : small (Z.pos r) A)
+                    (B : Z^sz) (_ : small (Z.pos r) B),
+                (eval A < eval m_enc
+                 -> eval B < eval m_enc
+                 -> small (Z.pos r) (f A B))))%Z }.
   Proof.
     exists (fun A B => sub (r:=r) (R_numlimbs:=sz) m_enc A B).
     abstract (
-        split; intros;
+        cbv zeta; intros; repeat apply conj; intros;
         unfold montgomery_to_F_gen; rewrite <- ?ModularArithmeticTheorems.F.of_Z_mul, <- ?ModularArithmeticTheorems.F.of_Z_sub;
         rewrite <- ?Z.mul_sub_distr_r;
         [ rewrite <- ModularArithmeticTheorems.F.eq_of_Z_iff, m_enc_correct_montgomery; push_Zmod; rewrite eval_sub_mod_N; pull_Zmod
-        | apply sub_bound ];
+        | apply sub_bound
+        | apply small_sub ];
         t_fin
       ).
   Defined.
@@ -170,15 +232,19 @@ Section with_args.
                  = (F.opp (montgomery_to_F_gen (eval A)))%F))
          /\ (forall (A : Z^sz) (_ : small (Z.pos r) A),
                 (eval A < eval m_enc
-                 -> 0 <= eval (f A) < eval m_enc)))%Z }.
+                 -> 0 <= eval (f A) < eval m_enc))
+         /\ (forall (A : Z^sz) (_ : small (Z.pos r) A),
+                (eval A < eval m_enc
+                 -> small (Z.pos r) (f A))))%Z }.
   Proof.
     exists (fun A => opp (r:=r) (R_numlimbs:=sz) m_enc A).
     abstract (
-        split; intros;
+        cbv zeta; intros; repeat apply conj; intros;
         unfold montgomery_to_F_gen; rewrite <- ?ModularArithmeticTheorems.F.of_Z_mul, <- ?F_of_Z_opp;
         rewrite <- ?Z.mul_opp_l;
         [ rewrite <- ModularArithmeticTheorems.F.eq_of_Z_iff, m_enc_correct_montgomery; push_Zmod; rewrite eval_opp_mod_N; pull_Zmod
-        | apply opp_bound ];
+        | apply opp_bound
+        | apply small_opp ];
         t_fin
       ).
   Defined.
@@ -193,11 +259,14 @@ Section with_args.
                  = montgomery_to_F_gen (eval A))))
          /\ (forall (A : Z^sz) (_ : small (Z.pos r) A),
                 (eval A < eval m_enc
-                 -> 0 <= eval (f A) < eval m_enc))%Z }.
+                 -> 0 <= eval (f A) < eval m_enc)
+         /\ (forall (A : Z^sz) (_ : small (Z.pos r) A),
+                (eval A < eval m_enc
+                 -> small (Z.pos r) (f A))))%Z }.
   Proof.
     exists (fun A => A).
     abstract (
-        split; eauto; split; auto;
+        cbv zeta; repeat (eauto || apply conj || intros);
         apply MontgomeryAPI.eval_small; auto; lia
       ).
   Defined.
@@ -231,318 +300,489 @@ Local Definition for_assumptions
 
 Print Assumptions for_assumptions.
 
-Ltac pose_m' modinv_fuel m r m' := (* (-m)⁻¹ mod r *)
-  pose_modinv modinv_fuel (-Z.pos m) (Z.pos r) m'.
-Ltac pose_r' modinv_fuel m r r' := (* r⁻¹ mod m *)
-  pose_modinv modinv_fuel (Z.pos r) (Z.pos m) r'.
+Section with_curves.
+  Import CurveParameters.CurveParameters.
+  Context (curve : CurveParameters)
+          (curve_sc : CurveParameterBaseSideConditions curve).
 
-Ltac pose_m'_correct m m' r m'_correct :=
-  pose_correct_if_Z
-    m'
-    ltac:(fun _ => constr:((Z.pos m * m') mod (Z.pos r) = (-1) mod Z.pos r))
-           m'_correct.
-Ltac pose_r'_correct m r r' r'_correct :=
-  pose_correct_if_Z
-    r'
-    ltac:(fun _ => constr:((Z.pos r * r') mod (Z.pos m) = 1))
-           r'_correct.
+  Local Notation modinv_fuel := curve.(modinv_fuel).
+  Local Notation m := curve.(m).
+  Local Notation r := curve.(r).
+  Local Notation base := curve.(base).
+  Local Notation sz := curve.(sz).
+  Local Notation s := curve.(s).
+  Local Notation c := curve.(c).
+  Local Notation carry_chains := curve.(carry_chains).
+  Local Notation coef := curve.(coef).
+  Local Notation mul_code := curve.(mul_code).
+  Local Notation square_code := curve.(square_code).
+  Local Notation sz_nonzero := curve_sc.(sz_nonzero).
+  Local Notation sz2_nonzero := curve_sc.(sz2_nonzero).
+  Local Notation s_nonzero := curve_sc.(s_nonzero).
+  Local Notation base_pos := curve_sc.(base_pos).
+  Local Notation sz_le_log2_m := curve_sc.(sz_le_log2_m).
+  Local Notation wt := curve.(wt).
+  Local Notation sz2 := curve.(sz2).
+  Local Notation half_sz := curve.(half_sz).
+  Local Notation sqrt_s := curve.(sqrt_s).
+  Local Notation bitwidth := curve.(bitwidth).
+  Local Notation m_enc := curve.(m_enc).
+  Local Notation wt0_1 := curve_sc.(wt0_1).
+  Local Notation wt_divides' := curve_sc.(wt_divides').
+  Local Notation wt_nonzero := curve_sc.(wt_nonzero).
+  Local Notation coef_mod := curve_sc.(coef_mod).
+  Local Notation m_correct := curve_sc.(m_correct).
+  Local Notation wt_divides_chains := curve_sc.(wt_divides_chains).
+  Local Notation sqrt_s_nonzero := curve_sc.(sqrt_s_nonzero).
+  Local Notation sqrt_s_correct := curve_sc.(sqrt_s_correct).
+  Local Notation fst_nat_divmod_sz_nonzero := curve_sc.(fst_nat_divmod_sz_nonzero).
+  Local Notation wt_divides := curve_sc.(wt_divides).
+  Local Notation wt_pos := curve_sc.(wt_pos).
+  Local Notation wt_multiples := curve_sc.(wt_multiples).
+  Local Notation c_small := curve_sc.(c_small).
+  Local Notation m_enc_bounded := curve_sc.(m_enc_bounded).
+  Local Notation m_correct_wt := curve_sc.(m_correct_wt).
+  Local Notation m_enc_correct := curve_sc.(m_enc_correct).
 
-Ltac pose_m_enc_correct_montgomery m sz r m_enc m_enc_correct_montgomery :=
-  cache_proof_with_type_by
-    (Z.pos m = MontgomeryAPI.eval (n:=sz) (Z.pos r) m_enc)
-    ltac:(vm_compute; reflexivity)
-           m_enc_correct_montgomery.
+  Local Notation exprT sz n szR :=
+    (((Tbase TZ^sz%nat)^n%nat -> Tbase TZ^szR%nat)%ctype)
+      (only parsing).
 
-Ltac pose_r'_pow_correct r' sz r m_enc r'_pow_correct :=
-  cache_proof_with_type_by
-    ((r' ^ Z.of_nat sz * Z.pos r ^ Z.of_nat sz) mod MontgomeryAPI.eval (n:=sz) (Z.pos r) m_enc = 1)
-    ltac:(vm_compute; reflexivity)
-           r'_pow_correct.
+  Let unoption_Expr_evar_package {sz szR}
+      n
+      (v : option
+             (Expr
+                (SmartMap.lift_flat_type
+                   Util.unextend_base_type
+                   ((Tbase Syntax.TZ ^ sz)^n)%ctype ->
+                 SmartMap.lift_flat_type
+                   Util.unextend_base_type
+                   (Tbase Syntax.TZ ^ szR))))
+    := cast_evar_package
+         (invert_Some v)
+         (Expr (exprT sz n szR)).
 
-Ltac pose_montgomery_to_F sz m r' montgomery_to_F :=
-  let v := (eval cbv [montgomery_to_F_gen] in (montgomery_to_F_gen sz m r')) in
-  cache_term v montgomery_to_F.
+  Import Crypto.Spec.ModularArithmetic.
 
-Ltac pose_r_big r r_big :=
-  cache_proof_with_type_by
-    (Z.pos r > 1)
-    ltac:(vm_compute; reflexivity)
-           r_big.
+  Record CurveParameterMontgomeryBaseSideConditions :=
+    { m' : modinv_evar_package modinv_fuel (-Z.pos m) (Z.pos r) (* (-m)⁻¹ mod r *);
+      r' : modinv_evar_package modinv_fuel (Z.pos r) (Z.pos m) (* r⁻¹ mod m *);
 
-Ltac pose_m_big m m_big :=
-  cache_proof_with_type_by
-    (1 < Z.pos m)
-    ltac:(vm_compute; reflexivity)
-           m_big.
+      r'_correct : (Z.pos r * val r') mod (Z.pos m) = 1
+      := evar_package_pf r';
 
-Ltac pose_m_enc_small sz r m_enc m_enc_small :=
-  cache_proof_with_type_by
-    (small (n:=sz) (Z.pos r) m_enc)
-    ltac:(pose (small_Decidable (n:=sz) (bound:=Z.pos r)); vm_decide_no_check)
-           m_enc_small.
+      m_enc_correct_montgomery' : vm_decide_package _;
+      m_enc_correct_montgomery : Z.pos m = MontgomeryAPI.eval (n:=sz) (Z.pos r) m_enc
+      := m_enc_correct_montgomery';
 
-Ltac pose_map_m_enc sz r m_enc map_m_enc :=
-  cache_proof_with_type_by
-    (Tuple.map (n:=sz) (Z.land (Z.pos r - 1)) m_enc = m_enc)
-    ltac:(pose (@dec_eq_prod); pose dec_eq_Z; vm_decide_no_check)
-           map_m_enc.
+      r'_pow_correct' : vm_decide_package _;
+      r'_pow_correct : (val r' ^ Z.of_nat sz * Z.pos r ^ Z.of_nat sz) mod MontgomeryAPI.eval (n:=sz) (Z.pos r) m_enc = 1
+      := r'_pow_correct';
 
-Ltac internal_pose_sig_by_eq ty sigl tac_eq id :=
-  cache_term_with_type_by
-    ty
-    ltac:(eapply (@sig_by_eq _ _ sigl _); tac_eq ())
-           id.
+      montgomery_to_F v := F.mul (F.of_Z m v) (F.of_Z m (val r'^Z.of_nat sz)%Z);
+      montgomery_of_F v := F.to_Z (v * F.of_Z m (r^Z.of_nat sz))%F;
 
-Import ModularArithmetic.
+      r_big' : vm_decide_package _;
+      r_big : Z.pos r > 1 := r_big';
 
-Local Ltac reduce_eq _ :=
-  cbv -[Definitions.Z.add_with_get_carry Definitions.Z.add_with_carry Definitions.Z.sub_with_get_borrow Definitions.Z.sub_with_borrow Definitions.Z.mul_split_at_bitwidth Definitions.Z.zselect runtime_add runtime_mul runtime_and runtime_opp runtime_lor Let_In].
+      m_big' : vm_decide_package _;
+      m_big : 1 < Z.pos m := m_big';
 
-Ltac pose_mul_ext r sz m m_enc r' r'_correct m' m'_correct m_enc_correct_montgomery r_big m_big m_enc_small montgomery_to_F mul_ext :=
-  internal_pose_sig_by_eq
-    { f:Z^sz -> Z^sz -> Z^sz
-    | let eval := MontgomeryAPI.eval (Z.pos r) in
-      (forall (A : Z^sz) (_ : small (Z.pos r) A)
-              (B : Z^sz) (_ : small (Z.pos r) B),
-          montgomery_to_F (eval (f A B))
-          = (montgomery_to_F (eval A) * montgomery_to_F (eval B))%F)
-      /\ (forall (A : Z^sz) (_ : small (Z.pos r) A)
-                 (B : Z^sz) (_ : small (Z.pos r) B),
-             (eval B < eval m_enc -> 0 <= eval (f A B) < eval m_enc)%Z) }
-    (@mul_ext_gen r sz m m_enc r' r'_correct m' m'_correct m_enc_correct_montgomery r_big m_big m_enc_small)
-    ltac:(fun _ => reduce_eq (); reflexivity)
-           mul_ext.
+      m_enc_small' : vm_decide_package _;
+      m_enc_small : small (n:=sz) (Z.pos r) m_enc
+      := @dec_bool _ _ m_enc_small';
 
-Ltac pose_add_ext r sz m m_enc r' m_enc_correct_montgomery r_big m_big m_enc_small montgomery_to_F add_ext :=
-  internal_pose_sig_by_eq
-    { f:Z^sz -> Z^sz -> Z^sz
-    | let eval := MontgomeryAPI.eval (Z.pos r) in
-      ((forall (A : Z^sz) (_ : small (Z.pos r) A)
-               (B : Z^sz) (_ : small (Z.pos r) B),
-           (eval A < eval m_enc
-            -> eval B < eval m_enc
-            -> montgomery_to_F (eval (f A B))
-               = (montgomery_to_F (eval A) + montgomery_to_F (eval B))%F))
-       /\ (forall (A : Z^sz) (_ : small (Z.pos r) A)
-                  (B : Z^sz) (_ : small (Z.pos r) B),
-              (eval A < eval m_enc
-               -> eval B < eval m_enc
-               -> 0 <= eval (f A B) < eval m_enc)))%Z }
-    (@add_ext_gen r sz m m_enc r' m_enc_correct_montgomery r_big m_big m_enc_small)
-    ltac:(fun _ => reduce_eq (); reflexivity)
-           add_ext.
+      map_m_enc' : vm_decide_package _;
+      map_m_enc : Tuple.map (n:=sz) (Z.land (Z.pos r - 1)) m_enc = m_enc
+      := @dec_bool _ _ map_m_enc';
+    }.
 
-Ltac pose_sub_ext r sz m m_enc r' m_enc_correct_montgomery r_big m_enc_small map_m_enc montgomery_to_F sub_ext :=
-  internal_pose_sig_by_eq
-    { f:Z^sz -> Z^sz -> Z^sz
-    | let eval := MontgomeryAPI.eval (Z.pos r) in
-      ((forall (A : Z^sz) (_ : small (Z.pos r) A)
-               (B : Z^sz) (_ : small (Z.pos r) B),
-           (eval A < eval m_enc
-            -> eval B < eval m_enc
-            -> montgomery_to_F (eval (f A B))
-               = (montgomery_to_F (eval A) - montgomery_to_F (eval B))%F))
-       /\ (forall (A : Z^sz) (_ : small (Z.pos r) A)
-                  (B : Z^sz) (_ : small (Z.pos r) B),
-              (eval A < eval m_enc
-               -> eval B < eval m_enc
-               -> 0 <= eval (f A B) < eval m_enc)))%Z }
-    (@sub_ext_gen r sz m m_enc r' m_enc_correct_montgomery r_big m_enc_small map_m_enc)
-    ltac:(fun _ => reduce_eq (); reflexivity)
-           sub_ext.
+  Context (curve_msc : CurveParameterMontgomeryBaseSideConditions).
 
-Ltac pose_opp_ext r sz m m_enc r' m_enc_correct_montgomery r_big m_enc_small map_m_enc montgomery_to_F opp_ext :=
-  internal_pose_sig_by_eq
-    { f:Z^sz -> Z^sz
-    | let eval := MontgomeryAPI.eval (Z.pos r) in
-      ((forall (A : Z^sz) (_ : small (Z.pos r) A),
-           (eval A < eval m_enc
-            -> montgomery_to_F (eval (f A))
-               = (F.opp (montgomery_to_F (eval A)))%F))
-       /\ (forall (A : Z^sz) (_ : small (Z.pos r) A),
-              (eval A < eval m_enc
-               -> 0 <= eval (f A) < eval m_enc)))%Z }
-    (@opp_ext_gen r sz m m_enc r' m_enc_correct_montgomery r_big m_enc_small map_m_enc)
-    ltac:(fun _ => reduce_eq (); reflexivity)
-           opp_ext.
+  Local Notation m'' := (val curve_msc.(m')).
+  Local Notation r'' := (val curve_msc.(r')).
+  Local Notation r'_correct' := curve_msc.(r'_correct).
+  Local Notation m_enc_correct_montgomery'' := curve_msc.(m_enc_correct_montgomery).
+  Local Notation r'_pow_correct'' := curve_msc.(r'_pow_correct).
+  Local Notation r_big'' := curve_msc.(r_big).
+  Local Notation m_big'' := curve_msc.(m_big).
+  Local Notation m_enc_small'' := curve_msc.(m_enc_small).
+  Local Notation map_m_enc'' := curve_msc.(map_m_enc).
+  Local Notation montgomery_to_F' := curve_msc.(montgomery_to_F).
+  Local Notation montgomery_of_F' := curve_msc.(montgomery_of_F).
 
-Ltac pose_carry_ext r sz m m_enc r' r_big montgomery_to_F carry_ext :=
-  internal_pose_sig_by_eq
-    { f:Z^sz -> Z^sz
-    | let eval := MontgomeryAPI.eval (Z.pos r) in
-      ((forall (A : Z^sz) (_ : small (Z.pos r) A),
-           (eval A < eval m_enc
-            -> montgomery_to_F (eval (f A))
-               = (montgomery_to_F (eval A))))
-       /\ (forall (A : Z^sz) (_ : small (Z.pos r) A),
-              (eval A < eval m_enc
-               -> 0 <= eval (f A) < eval m_enc)))%Z }
-    (@carry_ext_gen r sz m m_enc r' r_big)
-    ltac:(fun _ => reduce_eq (); reflexivity)
-           carry_ext.
+  Lemma montgomery_to_F_of_F v
+    : montgomery_to_F' (montgomery_of_F' v) = v.
+  Proof.
+    eapply montgomery_to_F_of_F_gen;
+      eauto using m_enc_correct_montgomery, r'_pow_correct.
+  Qed.
 
-Ltac pose_nonzero_ext r sz m m_enc r' m_enc_correct_montgomery r'_pow_correct r_big m_big montgomery_to_F nonzero_ext :=
-  internal_pose_sig_by_eq
-    { f:Z^sz -> Z
-    | let eval := MontgomeryAPI.eval (Z.pos r) in
-      forall (A : Z^sz) (_ : small (Z.pos r) A),
-        (eval A < eval m_enc
-         -> f A = 0 <-> (montgomery_to_F (eval A) = F.of_Z m 0))%Z }
-    (@nonzero_ext_gen r sz m m_enc r' m_enc_correct_montgomery r'_pow_correct r_big m_big)
-    ltac:(fun _ => reduce_eq (); reflexivity)
-           nonzero_ext.
+  Lemma montgomery_of_F_bounded (v : F m)
+    : 0 <= montgomery_of_F' v < Z.pos r ^ Z.of_nat sz.
+  Proof.
+    eapply montgomery_of_F_gen_bounded;
+      eauto using m_enc_correct_montgomery, r'_pow_correct, r_big, m_big, m_enc_small.
+  Qed.
 
-Ltac pose_mul_sig r sz montgomery_to_F mul_ext mul_sig :=
-  cache_term_with_type_by
-    { f:Z^sz -> Z^sz -> Z^sz
-    | let eval := MontgomeryAPI.eval (Z.pos r) in
-      forall (A : Z^sz) (_ : small (Z.pos r) A)
-             (B : Z^sz) (_ : small (Z.pos r) B),
-        montgomery_to_F (eval (f A B))
-        = (montgomery_to_F (eval A) * montgomery_to_F (eval B))%F }
-    ltac:(idtac;
-          let v := (eval cbv [proj1_sig mul_ext_gen mul_ext sig_by_eq] in (proj1_sig mul_ext)) in
-          (exists v);
-          abstract apply (proj2_sig mul_ext))
-           mul_sig.
+  Lemma m'_correct
+    : (Z.pos m * m'') mod (Z.pos r) = (-1) mod Z.pos r.
+  Proof.
+    pose proof (evar_package_pf curve_msc.(m')) as H; cbv beta in *.
+    generalize dependent m''; generalize m; generalize r; clear; intros r m m' H;
+      cbv [raw_evar_package] in *.
+    destruct (Z.eq_dec (Z.pos r) 1).
+    { destruct r as [[r|r|]|r|]; try congruence; try discriminate.
+      rewrite !Z.mod_1_r; reflexivity. }
+    change (-1) with (-(1)).
+    rewrite Z.mul_opp_l in H.
+    rewrite !Zdiv.Z_mod_nz_opp_full in *;
+      rewrite ?Z.mod_1_l by lia; try lia;
+        intro H';
+        rewrite Zdiv.Z_mod_zero_opp_full in H by assumption; congruence.
+  Qed.
 
-Ltac pose_mul_bounded r sz m_enc montgomery_to_F mul_ext mul_sig mul_bounded :=
-  cache_proof_with_type_by
-    (let eval := MontgomeryAPI.eval (Z.pos r) in
-     forall (A : Z^sz) (_ : small (Z.pos r) A)
-            (B : Z^sz) (_ : small (Z.pos r) B),
-       (eval B < eval m_enc
-        -> 0 <= eval (proj1_sig mul_sig A B) < eval m_enc)%Z)
-    ltac:(apply (proj2_sig mul_ext))
-           mul_bounded.
+  Local Notation Fencode := (@Positional.Fencode wt sz m (@modulo_cps) (@div_cps)).
 
+  Let encode_const : F m -> Expr (Unit -> (Tbase TZ)^sz)%ctype
+    := fun v var
+       => Abs
+            (fun _
+             => SmartMap.SmartPairf
+                  (flat_interp_untuple
+                     (T:=Tbase _)
+                     (Tuple.map
+                        (fun v => Op (OpConst v) TT)
+                        (Fencode v)))).
 
-Ltac pose_add_sig r sz m_enc montgomery_to_F add_ext add_sig :=
-  cache_term_with_type_by
-    { f:Z^sz -> Z^sz -> Z^sz
-    | let eval := MontgomeryAPI.eval (Z.pos r) in
-      forall (A : Z^sz) (_ : small (Z.pos r) A)
-             (B : Z^sz) (_ : small (Z.pos r) B),
-        (eval A < eval m_enc
-         -> eval B < eval m_enc
-         -> montgomery_to_F (eval (f A B))
-            = (montgomery_to_F (eval A) + montgomery_to_F (eval B))%F)%Z }
-    ltac:(idtac;
-          let v := (eval cbv [proj1_sig add_ext_gen add_ext sig_by_eq] in (proj1_sig add_ext)) in
-          (exists v);
-          abstract apply (proj2_sig add_ext))
-           add_sig.
+  Local Notation admit := (match AdmitAxiom.proof_admitted with end).
 
-Ltac pose_add_bounded r sz m_enc montgomery_to_F add_ext add_sig add_bounded :=
-  cache_proof_with_type_by
-    (let eval := MontgomeryAPI.eval (Z.pos r) in
-     (forall (A : Z^sz) (_ : small (Z.pos r) A)
-             (B : Z^sz) (_ : small (Z.pos r) B),
-         (eval A < eval m_enc
-          -> eval B < eval m_enc
-          -> 0 <= eval (proj1_sig add_sig A B) < eval m_enc))%Z)
-    ltac:(apply (proj2_sig add_ext))
-           add_bounded.
+  Record montgomery_side_conditions :=
+    {
+      not_freeze : vm_decide_package (curve.(freeze) = false);
+      tight_is_limb_width' : vm_decide_package _;
+      tight_is_limb_width : curve.(bounds_tight) = curve.(bounds_limb_widths)
+      := tight_is_limb_width';
+      loose_is_limb_width' : vm_decide_package _;
+      loose_is_limb_width : curve.(bounds_loose) = curve.(bounds_limb_widths)
+      := loose_is_limb_width';
+      limb_width_is_bitwidth' : vm_decide_package _;
+      limb_width_is_bitwidth : curve.(bounds_limb_widths) = curve.(bounds_bitwidths)
+      := limb_width_is_bitwidth';
 
+      vm_add_patterned := (fun ab => add_patterned r sz (m_enc, ab));
+      vm_sub_patterned := (fun ab => sub_patterned r sz (m_enc, ab));
+      vm_opp_patterned := (fun a => opp_patterned r sz (m_enc, a));
+      vm_nonzero_patterned := (nonzero_patterned sz);
+      vm_mul_patterned := (fun ab => redc_patterned r sz sz m'' (m_enc, ab));
 
-Ltac pose_sub_sig r sz m_enc montgomery_to_F sub_ext sub_sig :=
-  cache_term_with_type_by
-    { f:Z^sz -> Z^sz -> Z^sz
-    | let eval := MontgomeryAPI.eval (Z.pos r) in
-      forall (A : Z^sz) (_ : small (Z.pos r) A)
-             (B : Z^sz) (_ : small (Z.pos r) B),
-        (eval A < eval m_enc
-         -> eval B < eval m_enc
-         -> montgomery_to_F (eval (f A B))
-            = (montgomery_to_F (eval A) - montgomery_to_F (eval B))%F)%Z }
-    ltac:(idtac;
-          let v := (eval cbv [proj1_sig sub_ext_gen sub_ext sig_by_eq] in (proj1_sig sub_ext)) in
-          (exists v);
-          abstract apply (proj2_sig sub_ext))
-           sub_sig.
+      vm_compiled_preadd : vm_compute_evar_package_vm_large (Compiler.fill_first_of_pair_tupleZ (compiled_preadd r sz) m_enc);
+      vm_compiled_presub : vm_compute_evar_package_vm_large (Compiler.fill_first_of_pair_tupleZ (compiled_presub r sz) m_enc);
+      vm_compiled_preopp : vm_compute_evar_package_vm_large (Compiler.fill_first_of_pair_tupleZ (compiled_preopp r sz) m_enc);
+      vm_compiled_prenonzero : vm_compute_evar_package_vm_large (compiled_prenonzero sz);
+      vm_compiled_premul : vm_compute_evar_package_vm_large (Compiler.fill_first_of_pair_tupleZ (compiled_preredc' r sz sz m'') m_enc);
 
-Ltac pose_sub_bounded r sz m_enc montgomery_to_F sub_ext sub_sig sub_bounded :=
-  cache_proof_with_type_by
-    (let eval := MontgomeryAPI.eval (Z.pos r) in
-     (forall (A : Z^sz) (_ : small (Z.pos r) A)
-             (B : Z^sz) (_ : small (Z.pos r) B),
-         (eval A < eval m_enc
-          -> eval B < eval m_enc
-          -> 0 <= eval (proj1_sig sub_sig A B) < eval m_enc))%Z)
-    ltac:(apply (proj2_sig sub_ext))
-           sub_bounded.
+      evalF := montgomery_to_F';
+      evalZ := MontgomeryAPI.eval (n:=sz) (Z.pos r);
+      evalE := flat_interp_tuple (interp_base_type:=interp_base_type) (n:=sz) (T:=Tbase TZ);
+      preeval x := evalZ (evalE x);
+      eval x := evalF (preeval x);
 
+      zeroZ : vm_compute_evar_package_vm_small (encode_const 0%F);
+      oneZ : vm_compute_evar_package_vm_small (encode_const 1%F);
+      addZ : unoption_Expr_evar_package 2 (val vm_compiled_preadd);
+      subZ : unoption_Expr_evar_package 2 (val vm_compiled_presub);
+      oppZ : unoption_Expr_evar_package 1 (val vm_compiled_preopp);
+      nonzeroZ : unoption_Expr_evar_package 1 (val vm_compiled_prenonzero);
+      mulZ : unoption_Expr_evar_package 2 (val vm_compiled_premul);
+      val_squareZ : Expr (exprT sz 1 sz)
+      := fun var => Abs (fun x => invert_Abs (val mulZ var) (x, x));
 
-Ltac pose_opp_sig r sz m_enc montgomery_to_F opp_ext opp_sig :=
-  cache_term_with_type_by
-    { f:Z^sz -> Z^sz
-    | let eval := MontgomeryAPI.eval (Z.pos r) in
-      forall (A : Z^sz) (_ : small (Z.pos r) A),
-        (eval A < eval m_enc
-         -> montgomery_to_F (eval (f A))
-            = (F.opp (montgomery_to_F (eval A)))%F)%Z }
-    ltac:(idtac;
-          let v := (eval cbv [proj1_sig opp_ext_gen opp_ext sig_by_eq] in (proj1_sig opp_ext)) in
-          (exists v);
-          abstract apply (proj2_sig opp_ext))
-           opp_sig.
+      interp_addZ
+      : admit_package
+          (forall x y, evalE (Interp (val addZ) (x, y))
+                       = Compiler.do_apply (vm_add_patterned (evalE x, evalE y)))
+      := admit;
+      interp_subZ
+      : admit_package
+          (forall x y, evalE (Interp (val subZ) (x, y))
+                       = Compiler.do_apply (vm_sub_patterned (evalE x, evalE y)))
+      := admit;
+      interp_oppZ
+      : admit_package
+          (forall x, evalE (Interp (val oppZ) x)
+                     = Compiler.do_apply (vm_opp_patterned (evalE x)))
+      := admit;
+      interp_mulZ
+      : admit_package
+          (forall x y, evalE (Interp (val mulZ) (x, y))
+                       = Compiler.do_apply (vm_mul_patterned (evalE x, evalE y)))
+      := admit;
+      interp_nonzeroZ
+      : admit_package
+          (forall x, Interp (val nonzeroZ) x
+                     = Compiler.do_apply (vm_nonzero_patterned (evalE x)))
+      := admit;
 
-Ltac pose_opp_bounded r sz m_enc montgomery_to_F opp_ext opp_sig opp_bounded :=
-  cache_proof_with_type_by
-    (let eval := MontgomeryAPI.eval (Z.pos r) in
-     (forall (A : Z^sz) (_ : small (Z.pos r) A),
-         (eval A < eval m_enc
-          -> 0 <= eval (proj1_sig opp_sig A) < eval m_enc))%Z)
-    ltac:(apply (proj2_sig opp_ext))
-           opp_bounded.
+    }.
 
-Ltac pose_carry_sig r sz m_enc montgomery_to_F carry_ext carry_sig :=
-  cache_term_with_type_by
-    { f:Z^sz -> Z^sz
-    | let eval := MontgomeryAPI.eval (Z.pos r) in
-      forall (A : Z^sz) (_ : small (Z.pos r) A),
-        (eval A < eval m_enc
-         -> montgomery_to_F (eval (f A))
-            = (montgomery_to_F (eval A)))%Z }
-    ltac:(idtac;
-          let v := (eval cbv [proj1_sig carry_ext_gen carry_ext sig_by_eq] in (proj1_sig carry_ext)) in
-          (exists v);
-          abstract apply (proj2_sig carry_ext))
-           carry_sig.
+  Context (curve_scd : montgomery_side_conditions).
 
-Ltac pose_carry_bounded r sz m_enc montgomery_to_F carry_ext carry_sig carry_bounded :=
-  cache_proof_with_type_by
-    (let eval := MontgomeryAPI.eval (Z.pos r) in
-     (forall (A : Z^sz) (_ : small (Z.pos r) A),
-         (eval A < eval m_enc
-          -> 0 <= eval (proj1_sig carry_sig A) < eval m_enc))%Z)
-    ltac:(apply (proj2_sig carry_ext))
-           carry_bounded.
+  Local Notation evalZ' := curve_scd.(evalZ).
+  Local Notation evalE' := curve_scd.(evalE).
+  Local Notation evalF' := curve_scd.(evalF).
+  Local Notation eval' := curve_scd.(eval).
+  Local Notation preeval' := curve_scd.(preeval).
+  (*Local Notation zeroZ' := (val curve_scd.(zeroZ)).
+  Local Notation oneZ' := (val curve_scd.(oneZ)).*)
+  Local Notation addZ' := (val curve_scd.(addZ)).
+  Local Notation subZ' := (val curve_scd.(subZ)).
+  Local Notation oppZ' := (val curve_scd.(oppZ)).
+  Local Notation mulZ' := (val curve_scd.(mulZ)).
+  Local Notation nonzeroZ' := (val curve_scd.(nonzeroZ)).
+  (*Local Notation freezeZ' := (val curve_scd.(freezeZ)).*)
+  Local Notation squareZ' := curve_scd.(val_squareZ).
+
+  (*Lemma eval_zeroZ
+    : evalZ' zeroZ' = 0%F.
+  Proof. rewrite evar_package_pf_eq; apply proj2_sig. Qed.
+  Lemma eval_oneZ
+    : evalZ' oneZ' = 1%F.
+  Proof. rewrite evar_package_pf_eq; apply proj2_sig. Qed.*)
+
+  Local Ltac eval_t_whenever :=
+    repeat first [ progress cbn in *
+                 | progress intros
+                 | progress cbv [eval' preeval' evalZ' LetIn.Let_In evalF' montgomery_to_F montgomery_to_F_gen] in *
+                 | progress subst
+                 | progress destruct_head'_prod
+                 | progress destruct_head'_sig
+                 | exfalso; assumption
+                 | rewrite add_patterned_correct
+                 | rewrite sub_patterned_correct
+                 | rewrite redc_patterned_correct
+                 | rewrite opp_patterned_correct
+                 | rewrite nonzero_patterned_correct
+                 (*| rewrite freeze_patterned_correct*)
+                 | rewrite (evar_package_pf_eq curve_scd.(vm_add_patterned))
+                 | rewrite (evar_package_pf_eq curve_scd.(vm_sub_patterned))
+                 | rewrite (evar_package_pf_eq curve_scd.(vm_opp_patterned))
+                 | rewrite (evar_package_pf_eq curve_scd.(vm_mul_patterned))
+                 | rewrite (evar_package_pf_eq curve_scd.(vm_nonzero_patterned))
+                 (*| rewrite (evar_package_pf_eq curve_scd.(vm_freeze_patterned))*)
+                 | rewrite interp_addZ
+                 | rewrite interp_subZ
+                 | rewrite interp_oppZ
+                 | rewrite interp_mulZ
+                 | rewrite interp_nonzeroZ
+                 (*| rewrite interp_freezeZ*)
+                 | setoid_rewrite flat_interp_tuple_untuple
+                 | match goal with
+                   | [ |- ?x = ?x ] => reflexivity
+                   end
+                 | progress cbv [Interp] in * ].
+
+  Local Ltac eval_t_pose :=
+    pose proof wt_nonzero;
+    pose proof sz_nonzero;
+    pose proof sz2_nonzero;
+    pose proof wt0_1;
+    pose proof coef_mod;
+    pose proof div_mod;
+    pose proof s_nonzero;
+    pose proof m_correct;
+    pose proof wt_divides';
+    pose proof wt_divides_chains;
+    pose proof wt_divides;
+    pose proof wt_pos;
+    pose proof wt_multiples;
+    pose proof c_small;
+    pose proof m_enc_bounded;
+    pose proof div_correct; pose proof modulo_correct;
+    pose proof m'_correct;
+    pose proof r'_correct';
+    pose proof m_enc_correct_montgomery'';
+    pose proof r'_pow_correct'';
+    pose proof r_big'';
+    pose proof m_big'';
+    pose proof m_enc_small'';
+    pose proof map_m_enc''.
+  (*Local Ltac eval_t_pose_freeze :=
+    pose proof m_correct_wt;
+    pose proof m_enc_correct.*)
+
+  Local Ltac eval_t_fin :=
+    F_mod_eq;
+    repeat autounfold; repeat autorewrite with uncps push_id push_basesystem_eval;
+    try reflexivity; try eassumption.
 
 
-Ltac pose_nonzero_sig r sz m m_enc montgomery_to_F nonzero_ext nonzero_sig :=
-  cache_term_with_type_by
-    { f:Z^sz -> Z
-    | let eval := MontgomeryAPI.eval (Z.pos r) in
-      forall (A : Z^sz) (_ : small (Z.pos r) A),
-        (eval A < eval m_enc
-         -> f A = 0 <-> (montgomery_to_F (eval A) = F.of_Z m 0))%Z }
-    ltac:(idtac;
-          let v := (eval cbv [proj1_sig nonzero_ext_gen nonzero_ext sig_by_eq] in (proj1_sig nonzero_ext)) in
-          (exists v);
-          abstract apply (proj2_sig nonzero_ext))
-           nonzero_sig.
+  Local Ltac eval_t :=
+    eval_t_pose;
+    eval_t_whenever.
 
-Ltac pose_ring ring :=
-  (* FIXME: TODO *)
-  cache_term
-    I
-    ring.
+  Lemma addZ_gen
+    : forall ab,
+      (small (Z.pos r) (evalE' (fst ab))
+       -> small (Z.pos r) (evalE' (snd ab))
+       -> preeval' (fst ab) < evalZ' m_enc
+       -> preeval' (snd ab) < evalZ' m_enc
+       -> eval' (Interp addZ' ab) = (eval' (fst ab) + eval' (snd ab))%F)
+      /\ (small (Z.pos r) (evalE' (fst ab))
+          -> small (Z.pos r) (evalE' (snd ab))
+          -> preeval' (fst ab) < evalZ' m_enc
+          -> preeval' (snd ab) < evalZ' m_enc
+          -> 0 <= preeval' (Interp addZ' ab) < evalZ' m_enc)
+      /\ (small (Z.pos r) (evalE' (fst ab))
+          -> small (Z.pos r) (evalE' (snd ab))
+          -> preeval' (fst ab) < evalZ' m_enc
+          -> preeval' (snd ab) < evalZ' m_enc
+          -> small (Z.pos r) (evalE' (Interp addZ' ab))).
+  Proof.
+    pose proof (proj2_sig (@add_ext_gen r sz m m_enc r'' m_enc_correct_montgomery'' r_big'' m_big'' m_enc_small'')) as H.
+    cbv [add_ext_gen proj1_sig] in H.
+    eval_t.
+    destruct_head'_and; repeat apply conj; intros; eauto.
+  Qed.
 
-(* disable default unused things *)
-(*Ltac pose_carry_sig carry_sig :=
-  cache_term tt carry_sig.*)
-Ltac pose_freeze_sig freeze_sig :=
-  cache_term tt freeze_sig.
-Ltac pose_Mxzladderstep_sig Mxzladderstep_sig :=
-  cache_term tt Mxzladderstep_sig.
+  Definition eval_addZ ab := proj1 (addZ_gen ab).
+  Definition bounded_eval_addZ ab := proj2 (addZ_gen ab).
+
+  Lemma subZ_gen
+    : forall ab,
+      (small (Z.pos r) (evalE' (fst ab))
+       -> small (Z.pos r) (evalE' (snd ab))
+       -> preeval' (fst ab) < evalZ' m_enc
+       -> preeval' (snd ab) < evalZ' m_enc
+       -> eval' (Interp subZ' ab) = (eval' (fst ab) - eval' (snd ab))%F)
+      /\ (small (Z.pos r) (evalE' (fst ab))
+          -> small (Z.pos r) (evalE' (snd ab))
+          -> preeval' (fst ab) < evalZ' m_enc
+          -> preeval' (snd ab) < evalZ' m_enc
+          -> 0 <= preeval' (Interp subZ' ab) < evalZ' m_enc)
+      /\ (small (Z.pos r) (evalE' (fst ab))
+          -> small (Z.pos r) (evalE' (snd ab))
+          -> preeval' (fst ab) < evalZ' m_enc
+          -> preeval' (snd ab) < evalZ' m_enc
+          -> small (Z.pos r) (evalE' (Interp subZ' ab))).
+  Proof.
+    pose proof (proj2_sig (@sub_ext_gen r sz m m_enc r'' m_enc_correct_montgomery'' r_big'' m_enc_small'' map_m_enc'')) as H.
+    cbv [sub_ext_gen proj1_sig] in H.
+    eval_t.
+    destruct_head'_and; repeat apply conj; intros; eauto.
+  Qed.
+
+  Definition eval_subZ ab := proj1 (subZ_gen ab).
+  Definition bounded_eval_subZ ab := proj2 (subZ_gen ab).
+
+  Lemma oppZ_gen
+    : forall a,
+      (small (Z.pos r) (evalE' a)
+       -> preeval' a < evalZ' m_enc
+       -> eval' (Interp oppZ' a) = F.opp (eval' a))
+      /\ (small (Z.pos r) (evalE' a)
+          -> preeval' a < evalZ' m_enc
+          -> 0 <= preeval' (Interp oppZ' a) < evalZ' m_enc)
+      /\ (small (Z.pos r) (evalE' a)
+          -> preeval' a < evalZ' m_enc
+          -> small (Z.pos r) (evalE' (Interp oppZ' a))).
+  Proof.
+    pose proof (proj2_sig (@opp_ext_gen r sz m m_enc r'' m_enc_correct_montgomery'' r_big'' m_enc_small'' map_m_enc'')) as H.
+    cbv [opp_ext_gen proj1_sig] in H.
+    eval_t.
+    destruct_head'_and; repeat apply conj; intros; eauto.
+  Qed.
+
+  Definition eval_oppZ ab := proj1 (oppZ_gen ab).
+  Definition bounded_eval_oppZ ab := proj2 (oppZ_gen ab).
+
+  Lemma mulZ_gen
+    : forall ab,
+      (small (Z.pos r) (evalE' (fst ab))
+       -> small (Z.pos r) (evalE' (snd ab))
+       -> eval' (Interp mulZ' ab) = (eval' (fst ab) * eval' (snd ab))%F)
+      /\ (small (Z.pos r) (evalE' (fst ab))
+          -> small (Z.pos r) (evalE' (snd ab))
+          -> preeval' (snd ab) < evalZ' m_enc
+          -> 0 <= preeval' (Interp mulZ' ab) < evalZ' m_enc)
+      /\ (small (Z.pos r) (evalE' (fst ab))
+          -> small (Z.pos r) (evalE' (snd ab))
+          -> preeval' (fst ab) < evalZ' m_enc
+          -> preeval' (snd ab) < evalZ' m_enc
+          -> small (Z.pos r) (evalE' (Interp mulZ' ab))).
+  Proof.
+    pose proof (proj2_sig (@mul_ext_gen r sz m m_enc r'' r'_correct' m'' m'_correct m_enc_correct_montgomery'' r_big'' m_big'' m_enc_small'')) as H.
+    cbv [mul_ext_gen mul'_gen proj1_sig redc] in H.
+    eval_t.
+    destruct_head'_and; repeat apply conj; intros; eauto.
+  Qed.
+
+  Definition eval_mulZ ab := proj1 (mulZ_gen ab).
+  Definition bounded_eval_mulZ ab := proj2 (mulZ_gen ab).
+
+  Lemma eval_nonzeroZ_iff
+    : forall a,
+      small (Z.pos r) (evalE' a)
+      -> preeval' a < evalZ' m_enc
+      -> (Interp nonzeroZ' a = 0 <-> (eval' a = F.of_Z m 0)).
+  Proof.
+    pose proof (proj2_sig (@nonzero_ext_gen r sz m m_enc r'' m_enc_correct_montgomery'' r'_pow_correct'' r_big'' m_big'')) as H.
+    cbv [nonzero_ext_gen nonzero proj1_sig] in H.
+    eval_t.
+    eauto.
+  Qed.
+
+  Lemma eval_nonzeroZ
+    : forall a,
+      small (Z.pos r) (evalE' a)
+      -> preeval' a < evalZ' m_enc
+      -> (Interp nonzeroZ' a =? 0)
+         = (if Decidable.dec (eval' a = F.of_Z m 0) then true else false).
+  Proof.
+    intros a H0 H1.
+    destruct (eval_nonzeroZ_iff a H0 H1).
+    edestruct dec; destruct (Interp nonzeroZ' a =? 0) eqn:?; try reflexivity;
+      Z.ltb_to_lt;
+      exfalso; eauto.
+  Qed.
+
+  (*Local Definition ring_pkg : { T : _ & T }.
+  Proof.
+    eexists.
+    refine (Ring.ring_by_isomorphism
+              (F := F m)
+              (H := interp_flat_type interp_base_type (Tbase TZ^sz))
+              (phi := fun x => flat_interp_untuple (T:=Tbase TZ) (Positional.Fencode (div_cps:=@div_cps) (modulo_cps:=@modulo_cps) wt x))
+              (phi' := eval')
+              (zero := flat_interp_untuple (T:=Tbase TZ) zeroZ')
+              (one := flat_interp_untuple (T:=Tbase TZ) oneZ')
+              (add := fun x y => Interp carry_addZ' (x, y))
+              (sub := fun x y => Interp carry_subZ' (x, y))
+              (opp := Interp carry_oppZ')
+              (mul := fun x y => Interp carry_mulZ' (x, y))
+              (phi'_opp := eval_carry_oppZ)
+              _
+              _
+              _
+              _
+              _).
+    { abstract (
+          cbv [eval' evalZ']; setoid_rewrite flat_interp_tuple_untuple;
+          refine (Positional.Fdecode_Fencode_id
+                    (sz_nonzero := sz_nonzero)
+                    (div_mod := div_mod)
+                    wt wt0_1 wt_nonzero wt_divides');
+          eauto using @modulo_id, @div_id
+        ). }
+    { cbv [eval' evalZ']; intros; apply Positional.eq_Feq_iff. }
+    { abstract (cbv [eval']; setoid_rewrite flat_interp_tuple_untuple; rewrite eval_zeroZ; reflexivity). }
+    { abstract (cbv [eval']; setoid_rewrite flat_interp_tuple_untuple; rewrite eval_oneZ; reflexivity). }
+    { intros; apply eval_carry_addZ. }
+    { intros; apply eval_carry_subZ. }
+    { intros; apply eval_carry_mulZ. }
+  Defined.
+
+  Definition ring : _ /\ _ /\ _
+    := Eval cbv [ring_pkg projT2] in
+        projT2 ring_pkg.*)
+End with_curves.
