src/Specific/X25519/C64/Synthesis.v
@@ -1,9 +1,113 @@
-Require Import Crypto.Specific.Framework.SynthesisFramework.
+Require Import Crypto.Specific.Framework.Pipeline.
 Require Import Crypto.Specific.X25519.C64.CurveParameters.
 
-Module P <: PrePackage.
-  Definition package : Tag.Context.
-  Proof. make_Synthesis_package curve extra_prove_mul_eq extra_prove_square_eq. Defined.
-End P.
+Definition curve := CurveParameters.CurveParameters.fill_CurveParameters curve.
 
-Module Export S := PackageSynthesis P.
+  Lemma rew_impl (a b : bool) : (if a then b else true) = implb a b.
+  Proof. destruct a, b; reflexivity. Qed.
+Definition package : SynthesisOutput curve.
+Proof.
+  Require Import Crypto.Util.Tactics.Not.
+  Require Import Crypto.Specific.Framework.ArithmeticSynthesis.Base.
+  Require Import Crypto.Util.SideConditions.CorePackages.
+  Require Import Crypto.Util.SideConditions.Autosolve.
+  Set Ltac Profiling.
+  repeat lazymatch goal with
+         | [ |- SynthesisOutput ?e ]
+           => not has_evar e; unshelve eapply @Pipeline
+         | [ |- CurveParameterBaseSideConditions ?e ]
+           => not has_evar e; unshelve econstructor
+         end.
+  Time autosolve ltac:(fun _ => fail).
+  repeat lazymatch goal with
+         | [ |- PipelineSideConditions ?e _ ]
+           => not has_evar e; unshelve econstructor
+         | [ |- Solinas.solinas_side_conditions ?e ]
+           => not has_evar e; unshelve econstructor
+         end.
+  Notation vm_ev := (ReductionPackages.vm_compute_evar_package_gen _).
+  Notation cast_ev := (ReductionPackages.cast_evar_package _ _).
+  Notation option_ev := (ReductionPackages.option_evar_rel_package _ _ _ _).
+  Notation vm_dec := (ReductionPackages.vm_decide_package _).
+  Notation ring_pkg := (RingPackage.eq_by_Zring_prod_package _).
+  Import Compilers.Syntax.
+  48-51:simpl @CurveParameters.CurveParameters.sz;
+    cbv [Syntax.tuple Syntax.tuple' option_map val].
+  Time autosolve ltac:(fun _ => fail).
+  Time autosolve ltac:(fun _ => fail).
+  Time autosolve ltac:(fun _ => fail).
+  Time autosolve ltac:(fun _ => fail).
+  Time autosolve ltac:(fun _ => fail).
+  Time autosolve ltac:(fun _ => fail).
+  Time autosolve ltac:(fun _ => fail).
+  Time autosolve ltac:(fun _ => fail).
+  Time autosolve ltac:(fun _ => fail).
+  Time autosolve ltac:(fun _ => fail).
+  Time autosolve ltac:(fun _ => fail).
+  Time autosolve ltac:(fun _ => fail).
+  Time autosolve ltac:(fun _ => fail).
+  Time autosolve ltac:(fun _ => fail).
+  Time autosolve ltac:(fun _ => fail).
+  Time autosolve ltac:(fun _ => fail).
+  Time autosolve ltac:(fun _ => fail).
+  Time autosolve ltac:(fun _ => fail).
+  Time autosolve ltac:(fun _ => fail).
+  Time autosolve ltac:(fun _ => fail).
+  Time autosolve ltac:(fun _ => fail).
+  Time autosolve ltac:(fun _ => fail).
+  Time autosolve ltac:(fun _ => fail).
+  Time autosolve ltac:(fun _ => fail).
+  Time autosolve ltac:(fun _ => fail).
+  Time autosolve ltac:(fun _ => fail).
+  Time autosolve ltac:(fun _ => fail).
+  Time autosolve ltac:(fun _ => fail).
+  Time autosolve ltac:(fun _ => fail).
+  Time autosolve ltac:(fun _ => fail).
+  Time autosolve ltac:(fun _ => fail).
+  Time autosolve ltac:(fun _ => fail).
+  Time autosolve ltac:(fun _ => fail).
+  Time autosolve ltac:(fun _ => fail).
+  Time autosolve ltac:(fun _ => fail).
+  Time autosolve ltac:(fun _ => fail).
+  { Require Import Crypto.Compilers.Reify.
+    Require Import Crypto.Compilers.Z.Reify.
+    Require Import Crypto.Util.SideConditions.Autosolve.
+    Time autosolve ltac:(fun _ => fail). }
+  { Time autosolve ltac:(fun _ => fail). }
+  { Time autosolve ltac:(fun _ => fail). }
+  { Time autosolve ltac:(fun _ => fail). }
+  { Time autosolve ltac:(fun _ => fail). }
+  { Time autosolve ltac:(fun _ => fail). }
+  { Time autosolve ltac:(fun _ => fail). }
+  { Time autosolve ltac:(fun _ => fail). }
+  { Time autosolve ltac:(fun _ => fail). }
+  { Time autosolve ltac:(fun _ => fail). }
+  { Time autosolve ltac:(fun _ => fail). }
+  { Time autosolve ltac:(fun _ => fail). }
+  { Time autosolve ltac:(fun _ => fail). }
+  { Time autosolve ltac:(fun _ => fail). }
+  { Time autosolve ltac:(fun _ => fail). }
+  { Time
+      repeat lazymatch goal with
+             | [ |- SynthesisOutput ?e ]
+               => not has_evar e; unshelve eapply @Pipeline
+             | [ |- CurveParameterBaseSideConditions ?e ]
+               => not has_evar e; unshelve econstructor
+             | [ |- PipelineSideConditions ?e _ ]
+               => not has_evar e; unshelve econstructor
+             | [ |- Solinas.solinas_side_conditions ?e ]
+               => not has_evar e; unshelve econstructor
+             | [ |- BoundsPipeline.BoundsSideConditions ?e ]
+               => not has_evar e; unshelve econstructor
+             end.
+    { Time autosolve ltac:(fun _ => fail). }
+    { Time autosolve ltac:(fun _ => fail). }
+    { Time autosolve ltac:(fun _ => BoundsPipeline.autosolve ltac:(fun _ => fail)). }
+    { Time autosolve ltac:(fun _ => BoundsPipeline.autosolve ltac:(fun _ => fail)). }
+    { Time autosolve ltac:(fun _ => BoundsPipeline.autosolve ltac:(fun _ => fail)). }
+    { Time autosolve ltac:(fun _ => BoundsPipeline.autosolve ltac:(fun _ => fail)). }
+    { Time autosolve ltac:(fun _ => BoundsPipeline.autosolve ltac:(fun _ => fail)). }
+    { Time autosolve ltac:(fun _ => BoundsPipeline.autosolve ltac:(fun _ => fail)). }
+    { Time autosolve ltac:(fun _ => BoundsPipeline.autosolve ltac:(fun _ => fail)). }
+    { vm_compute; reflexivity. } }
+Time Defined.
