src/Specific/montgomery32_2e256m2e224p2e192p2e96m1_8limbs/Synthesis.v
@@ -1,9 +1,179 @@
-Require Import Crypto.Specific.Framework.SynthesisFramework.
+Require Import Crypto.Specific.Framework.Pipeline.
 Require Import Crypto.Specific.montgomery32_2e256m2e224p2e192p2e96m1_8limbs.CurveParameters.
 
-Module P <: PrePackage.
+Definition curve := CurveParameters.CurveParameters.fill_CurveParameters curve.
+
+  Require Import Crypto.Util.Tactics.Not.
+  Require Import Crypto.Specific.Framework.ArithmeticSynthesis.Base.
+  Require Import Crypto.Util.SideConditions.CorePackages.
+  Require Import Crypto.Util.SideConditions.Autosolve.
+  Notation vm_ev := (ReductionPackages.vm_compute_evar_package_gen _).
+  Notation cast_ev := (ReductionPackages.cast_evar_package _ _).
+  Notation option_ev := (ReductionPackages.option_evar_rel_package _ _ _ _).
+  Notation vm_dec := (ReductionPackages.vm_decide_package _).
+  Notation ring_pkg := (RingPackage.eq_by_Zring_prod_package _).
+  Import Compilers.Syntax.
+
+  Definition package : SynthesisOutput curve.
+Proof.
+  Set Ltac Profiling.
+  Import Head.
+  Ltac myfail := idtac "fail"; lazymatch goal with |- ?G => let h := head G in idtac h; idtac G end; fail.
+  repeat lazymatch goal with
+         | [ |- SynthesisOutput ?e ]
+           => not has_evar e; unshelve eapply @Pipeline
+         | [ |- CurveParameterBaseSideConditions ?e ]
+           => not has_evar e; unshelve econstructor
+         end.
+  Time autosolve ltac:(fun _ => myfail).
+  repeat lazymatch goal with
+         | [ |- PipelineSideConditions ?e _ ]
+           => not has_evar e; unshelve econstructor
+         | [ |- Solinas.solinas_side_conditions ?e ]
+           => not has_evar e; unshelve econstructor
+         | [ |- Montgomery.montgomery_side_conditions ?e ]
+           => not has_evar e; unshelve econstructor
+         | [ |- Montgomery.CurveParameterMontgomeryBaseSideConditions ?e ]
+           => not has_evar e; unshelve econstructor
+         end.
+  Time autosolve ltac:(fun _ => myfail).
+  Time autosolve ltac:(fun _ => myfail).
+  Time autosolve ltac:(fun _ => myfail).
+  Time autosolve ltac:(fun _ => myfail).
+  Time autosolve ltac:(fun _ => myfail).
+  Time autosolve ltac:(fun _ => myfail).
+  Time autosolve ltac:(fun _ => myfail).
+  Time autosolve ltac:(fun _ => myfail).
+  repeat lazymatch goal with
+         | [ |- PipelineSideConditions ?e _ ]
+           => not has_evar e; unshelve econstructor
+         | [ |- Solinas.solinas_side_conditions ?e ]
+           => not has_evar e; unshelve econstructor
+         | [ |- Montgomery.montgomery_side_conditions ?e ]
+           => not has_evar e; unshelve econstructor
+         | [ |- Montgomery.CurveParameterMontgomeryBaseSideConditions ?e ]
+           => not has_evar e; unshelve econstructor
+         end.
+  Time autosolve ltac:(fun _ => myfail).
+  Time autosolve ltac:(fun _ => myfail).
+  Time autosolve ltac:(fun _ => myfail).
+  Time autosolve ltac:(fun _ => myfail).
+  Time autosolve ltac:(fun _ => myfail).
+  { Time autosolve ltac:(fun _ => myfail). }
+  { Time autosolve ltac:(fun _ => myfail). }
+  { Time autosolve ltac:(fun _ => myfail). }
+  { Time autosolve ltac:(fun _ => myfail). }
+  { Time autosolve ltac:(fun _ => myfail). }
+  { Time autosolve ltac:(fun _ => myfail). }
+  { Time autosolve ltac:(fun _ => myfail). }
+  { Time autosolve ltac:(fun _ => myfail). }
+  { Time autosolve ltac:(fun _ => myfail). }
+  { Time autosolve ltac:(fun _ => myfail). }
+  { Time autosolve ltac:(fun _ => myfail). }
+  { Time
+      repeat lazymatch goal with
+             | [ |- SynthesisOutput ?e ]
+               => not has_evar e; unshelve eapply @Pipeline
+             | [ |- CurveParameterBaseSideConditions ?e ]
+               => not has_evar e; unshelve econstructor
+             | [ |- PipelineSideConditions ?e _ ]
+               => not has_evar e; unshelve econstructor
+             | [ |- Solinas.solinas_side_conditions ?e ]
+               => not has_evar e; unshelve econstructor
+             | [ |- Montgomery.montgomery_side_conditions ?e ]
+               => not has_evar e; unshelve econstructor
+             | [ |- Montgomery.CurveParameterMontgomeryBaseSideConditions ?e ]
+               => not has_evar e; unshelve econstructor
+             | [ |- BoundsPipeline.BoundsSideConditions ?e ]
+               => not has_evar e; unshelve econstructor
+             end.
+    { idtac "here".
+      { Time autosolve ltac:(fun _ => myfail). } }
+    { Time autosolve ltac:(fun _ => myfail). }
+    { Time autosolve ltac:(fun _ => BoundsPipeline.autosolve ltac:(fun _ => myfail)). }
+    { Time autosolve ltac:(fun _ => BoundsPipeline.autosolve ltac:(fun _ => myfail)). }
+    { Time autosolve ltac:(fun _ => BoundsPipeline.autosolve ltac:(fun _ => myfail)). }
+    { Time autosolve ltac:(fun _ => BoundsPipeline.autosolve ltac:(fun _ => myfail)). }
+    { Time autosolve ltac:(fun _ => BoundsPipeline.autosolve ltac:(fun _ => myfail)). }
+    { Time autosolve ltac:(fun _ => BoundsPipeline.autosolve ltac:(fun _ => myfail)). }
+    { Time autosolve ltac:(fun _ => BoundsPipeline.autosolve ltac:(fun _ => myfail)). }
+    { Time autosolve ltac:(fun _ => BoundsPipeline.autosolve ltac:(fun _ => myfail)). } }
+  Show Ltac Profile.
+  Time Defined.
+Time Print Assumptions package.
+
+
+Definition zero := Eval lazy in zero (opsW package).
+Definition one := Eval lazy in one (opsW package).
+Definition add := Eval lazy in add (opsW package).
+Definition sub := Eval lazy in sub (opsW package).
+Definition opp := Eval lazy in opp (opsW package).
+Definition carry_mul := Eval lazy in carry_mul (opsW package).
+Definition carry_square := Eval lazy in carry_square (opsW package).
+Definition nonzero := Eval lazy in nonzero (opsW package).
+Definition freeze := Eval lazy in freeze (opsW package).
+
+Require Import Framework.IntegrationTestDisplayCommon.
+
+Print zero.
+Print one.
+Print add.
+Print sub.
+Print opp.
+Print carry_mul.
+Print carry_square.
+Print nonzero.
+Print freeze.
+
+(*
+Require Import CNotations.
+Print SynthesisOutput.
+Check opsW package.
+Print SynthesisOutputOps.
+Goal True.
+  pose (sub (opsW package)) as e.
+  Time lazy in e.
+  Time Print Assumptions package.
+  simple refine (let v := carry (opsZ (_ : SynthesisOutput curve)) in
+                 _).
+  clear e.
+  unshelve eapply @Pipeline.
+  autosolve ltac:(fun _ => fail).
+  unshelve econstructor.
+  unshelve econstructor.
+  Focus 11.
+  cbv [carry opsZ Pipeline] in v.
+  cbv [CurveParameters.CurveParameters.montgomery curve ] in v.
+  cbv [curve_sc] in v.
+  cbv [MontgomeryBoundsPipelineInputSideConditions.ropsZ] in v.
+  cbv [rT] in v.
+  Timeout 2 lazy in v.
+  cbv [CurveParameters.CurveParameters.sz] in v.
+  Print BoundsPipeline.BoundsPipeline.
+  cbv [BoundsPipeline.BoundsPipeline] in v.
+compute in v.
+  hnf in v.
+  Locate
+  Eval hnf in @Pipeline curve _ _. {| mropsZ := _ |}.
+  Time vm_compute in e.
+  idtac.
+  Unset Silent.
+  Time Show.
+  Time idtac.
+  pose (sub (opsW package)) as e.
+  Time cbv [sub opsW package] in e.
+  idtac.
+  Unset Silent.
+  Time Show.
+  Time idtac.
+  Notation hidden := (sub _).
+
+Time Compute sub (opsW package).
+(*Module P <: PrePackage.
   Definition package : Tag.Context.
   Proof. make_Synthesis_package curve extra_prove_mul_eq extra_prove_square_eq. Defined.
 End P.
 
 Module Export S := PackageSynthesis P.
+*)
+*)
