src/Arithmetic/Compiled/Saturated/Freeze.v
@@ -1,0 +1,27 @@
+Require Import Coq.ZArith.BinInt.
+Require Import Crypto.Arithmetic.Saturated.FreezeUnfolder.
+Require Import Crypto.Arithmetic.Saturated.Freeze.
+Require Import Crypto.Arithmetic.Compiled.Compiler.
+
+Definition freeze_patterned (weight : nat -> Z) (n : nat) (mask : Z) (xy : Tuple.tuple Z n * Tuple.tuple Z n)
+  := do_pattern_strip (@freeze_cps weight n mask (fst xy) (snd xy) _ id).
+
+Definition freeze_patterned_correct wt n mask xy
+  : do_apply (freeze_patterned wt n mask xy)
+    = @freeze_cps wt n mask (fst xy) (snd xy) _ id
+  := eq_refl.
+
+Definition compiled_prefreeze_sig (weight : nat -> Z) (n : nat) (mask : Z)
+  : { t : _ & t }.
+Proof.
+  let freeze_cps := (eval cbv delta [freeze_cps] in freeze_cps) in
+  do_compile_sig
+    (fun n T f weight mask xy => @freeze_cps weight n mask (fst xy) (snd xy) T f)
+    uconstr:(fun t xy => t n weight mask xy).
+Defined.
+
+Definition compiled_prefreeze' wt n mask
+  := Eval cbv [projT2 projT1 compiled_prefreeze_sig] in
+      projT2 (compiled_prefreeze_sig wt n mask).
+
+Time Definition compiled_prefreeze := compiler_prered compiled_prefreeze'.
