src/Arithmetic/KaratsubaUnfolder.v
@@ -1,0 +1,37 @@
+Require Import Crypto.Arithmetic.CoreUnfolder.
+Require Import Crypto.Arithmetic.Karatsuba.
+
+(**
+<<
+#!/bin/bash
+for i in karatsuba_mul_cps karatsuba_mul goldilocks_mul_cps goldilocks_mul; do
+    echo "Definition ${i}_sig := parameterize_sig (@${i}).";
+    echo "Definition ${i} := parameterize_from_sig ${i}_sig.";
+    echo "Definition ${i}_eq := parameterize_eq ${i} ${i}_sig.";
+    echo "Hint Unfold ${i} : basesystem_partial_evaluation_unfolder.";
+    echo "Hint Rewrite <- ${i}_eq : pattern_runtime."; echo "";
+done
+>> *)
+Definition karatsuba_mul_cps_sig := parameterize_sig (@karatsuba_mul_cps).
+Definition karatsuba_mul_cps := parameterize_from_sig karatsuba_mul_cps_sig.
+Definition karatsuba_mul_cps_eq := parameterize_eq karatsuba_mul_cps karatsuba_mul_cps_sig.
+Hint Unfold karatsuba_mul_cps : basesystem_partial_evaluation_unfolder.
+Hint Rewrite <- karatsuba_mul_cps_eq : pattern_runtime.
+
+Definition karatsuba_mul_sig := parameterize_sig (@karatsuba_mul).
+Definition karatsuba_mul := parameterize_from_sig karatsuba_mul_sig.
+Definition karatsuba_mul_eq := parameterize_eq karatsuba_mul karatsuba_mul_sig.
+Hint Unfold karatsuba_mul : basesystem_partial_evaluation_unfolder.
+Hint Rewrite <- karatsuba_mul_eq : pattern_runtime.
+
+Definition goldilocks_mul_cps_sig := parameterize_sig (@goldilocks_mul_cps).
+Definition goldilocks_mul_cps := parameterize_from_sig goldilocks_mul_cps_sig.
+Definition goldilocks_mul_cps_eq := parameterize_eq goldilocks_mul_cps goldilocks_mul_cps_sig.
+Hint Unfold goldilocks_mul_cps : basesystem_partial_evaluation_unfolder.
+Hint Rewrite <- goldilocks_mul_cps_eq : pattern_runtime.
+
+Definition goldilocks_mul_sig := parameterize_sig (@goldilocks_mul).
+Definition goldilocks_mul := parameterize_from_sig goldilocks_mul_sig.
+Definition goldilocks_mul_eq := parameterize_eq goldilocks_mul goldilocks_mul_sig.
+Hint Unfold goldilocks_mul : basesystem_partial_evaluation_unfolder.
+Hint Rewrite <- goldilocks_mul_eq : pattern_runtime.
