src/Specific/Framework/Pipeline.v
@@ -1,0 +1,164 @@
+Require Import Coq.ZArith.BinIntDef.
+Require Import Coq.omega.Omega.
+Require Import Coq.micromega.Lia.
+Require Import Crypto.Arithmetic.Core. Import B.
+Require Import Crypto.Arithmetic.PrimeFieldTheorems.
+Require Import Crypto.Compilers.Z.Bounds.Pipeline.Definition.
+Require Import Crypto.Compilers.Z.Bounds.Pipeline.ReflectiveTactics.
+Require Import Crypto.Compilers.Syntax.
+Require Import Crypto.Compilers.SmartMap.
+Require Import Crypto.Compilers.Tuple.
+Require Import Crypto.Compilers.ExprInversion.
+Require Import Crypto.Compilers.Z.Syntax.Util.
+Require Import Crypto.Compilers.Z.Syntax.
+Require Import Crypto.Compilers.Tuple.
+Require Import Crypto.Util.SideConditions.CorePackages.
+Require Import Crypto.Util.SideConditions.ReductionPackages.
+Require Import Crypto.Specific.Framework.CurveParameters.
+Require Import Crypto.Specific.Framework.ArithmeticSynthesis.Base.
+Require Import Crypto.Specific.Framework.ArithmeticSynthesis.Solinas.
+Require Import Crypto.Specific.Framework.ArithmeticSynthesis.Montgomery.
+Require Export Crypto.Specific.Framework.OutputType.
+Require Import Crypto.Specific.Framework.MontgomeryBoundsPipelineInputSideConditions.
+Require Import Crypto.Specific.Framework.SolinasBoundsPipelineInputSideConditions.
+Require Import Crypto.Specific.Framework.BoundsPipelineInputSideConditions.
+Require Import Crypto.Specific.Framework.BoundsPipeline.
+Require Import Crypto.Util.Notations.
+Require Import Crypto.Util.Tactics.BreakMatch.
+Require Import Crypto.Util.Tactics.DestructHead.
+Require Import Crypto.Util.ZUtil.Tactics.PeelLe.
+Require Import Crypto.Util.ZUtil.Tactics.ReplaceNegWithPos.
+Require Import Crypto.Util.ListUtil.
+Require Import Crypto.Util.ZUtil.
+Import CurveParameters.Notations.
+
+Local Set Implicit Arguments.
+Local Coercion Z.to_nat : Z >-> nat.
+Local Notation interp_flat_type := (interp_flat_type interp_base_type).
+
+Section gen.
+  Context (curve : CurveParameters.CurveParameters)
+          (curve_sc' : vm_decide_package (CurveParameterBaseSideConditions_bool curve = true)).
+
+  Definition curve_sc
+    := CurveParameterBaseSideConditions_bool_correct curve curve_sc'.
+
+  Record SolinasPipelineSC :=
+    {
+      ssc :> solinas_side_conditions curve_sc;
+      sropsZ := SolinasBoundsPipelineInputSideConditions.ropsZ ssc;
+      sP_extra := SolinasBoundsPipelineInputSideConditions.P_extra curve;
+      sHP_extra := SolinasBoundsPipelineInputSideConditions.HP_extra ssc;
+      scurve_scib := SolinasBoundsPipelineInputSideConditions.curve_scib ssc;
+      sbounds :> BoundsSideConditions sropsZ;
+    }.
+
+  Record MontgomeryPipelineSC :=
+    {
+      mscb :> CurveParameterMontgomeryBaseSideConditions curve;
+      msc :> montgomery_side_conditions mscb;
+      mropsZ := MontgomeryBoundsPipelineInputSideConditions.ropsZ msc;
+      mP_extra := MontgomeryBoundsPipelineInputSideConditions.P_extra curve;
+      mHP_extra := MontgomeryBoundsPipelineInputSideConditions.HP_extra curve_sc msc;
+      mcurve_scib := MontgomeryBoundsPipelineInputSideConditions.curve_scib curve_sc msc;
+      mbounds :> BoundsSideConditions mropsZ;
+    }.
+
+  Definition PipelineSideConditions
+    := if curve.(montgomery)
+       then MontgomeryPipelineSC
+       else SolinasPipelineSC.
+
+  Context (sc : PipelineSideConditions).
+
+  Definition Pipeline : SynthesisOutput curve.
+  Proof.
+    hnf in sc.
+    pose curve_sc.
+    (destruct curve.(montgomery) eqn:?);
+      destruct sc;
+      unshelve eapply @BoundsPipeline; assumption.
+  Defined.
+End gen.
+
+(** Overwrite the [RBPipelineSideConditions_unfold] stub with the
+    things we should actually unfold, now that we have access to
+    them. *)
+Ltac RBPipelineSideConditions_unfold ::=
+  cbv [val
+         Option.invert_Some Build_evard_package
+         SolinasBoundsPipelineInputSideConditions.ropsZ
+         (* OutputType *)
+         OutputType.zero
+         OutputType.one
+         OutputType.add
+         OutputType.sub
+         OutputType.carry_mul
+         OutputType.carry_square
+         OutputType.opp
+         OutputType.carry
+         OutputType.freeze
+         OutputType.nonzero
+         OutputType.carry_add
+         OutputType.carry_sub
+         OutputType.carry_opp
+         (* Solinas *)
+         Solinas.not_montgomery
+         Solinas.vm_add_patterned
+         Solinas.vm_sub_patterned
+         Solinas.vm_mul_patterned
+         Solinas.vm_opp_patterned
+         Solinas.vm_reduce_patterned
+         Solinas.vm_reduce_patterned_sz_sz
+         Solinas.vm_reduce_patterned_sz_1p5
+         Solinas.vm_chained_carries_reduce_patterned
+         Solinas.vm_karatsuba_mul_patterned
+         Solinas.vm_goldilocks_mul_patterned
+         Solinas.vm_freeze_patterned
+         Solinas.vm_compiled_preadd
+         Solinas.vm_compiled_presub
+         Solinas.vm_compiled_premul
+         Solinas.vm_compiled_preopp
+         Solinas.vm_compiled_prereduce
+         Solinas.vm_compiled_prereduce_sz_sz
+         Solinas.vm_compiled_prereduce_sz_1p5
+         Solinas.vm_compiled_prechained_carries_reduce
+         Solinas.vm_compiled_prekaratsuba_mul
+         Solinas.vm_compiled_pregoldilocks_mul
+         Solinas.vm_compiled_prefreeze
+         Solinas.mul_code_correct
+         Solinas.square_code_correct
+         Solinas.evalZ
+         Solinas.evalZ2
+         Solinas.evalZ1p5
+         Solinas.evalE
+         Solinas.evalE2
+         Solinas.evalE1p5
+         Solinas.eval
+         Solinas.eval2
+         Solinas.eval1p5
+         Solinas.mul_code_casted
+         Solinas.square_code_casted
+         Solinas.mul_codeZ
+         Solinas.square_codeZ
+         Solinas.zeroZ
+         Solinas.oneZ
+         Solinas.addZ
+         Solinas.subZ
+         Solinas.oppZ
+         Solinas.carryZ
+         Solinas.reduceZ
+         Solinas.reduceZ_sz_sz
+         Solinas.reduceZ_sz_1p5
+         Solinas.premulZ
+         Solinas.val_presquareZ
+         Solinas.prekaratsuba_mulZ
+         Solinas.pregoldilocks_mulZ
+         Solinas.val_prekaratsuba_squareZ
+         Solinas.val_pregoldilocks_squareZ
+         Solinas.freezeZ
+         Solinas.carry_mulZ
+         Solinas.carry_squareZ
+         Solinas.carry_addZ
+         Solinas.carry_subZ
+         Solinas.carry_oppZ].
